UNSTABLE3

Propositional.v
@@ -1,2 +1,62 @@
 (* Here will be theorems about propositional logic.
 Then I'll decide how to unite it with the rest. *)
+
+Require Export Coq.Vectors.Vector.
+Require Import Coq.Structures.Equalities.
+Add LoadPath "/home/user/0my/GITHUB/VerifiedMathFoundations/library".
+
+Require Poly.
+Export Poly.ModProp.
+
+Module  Formulas_mod (PropVars : UsualDecidableTypeFull).
+
+Inductive Fo :=
+ |Atom (p:PropVars.t) :> Fo
+ |Bot :Fo
+ |Conj:Fo->Fo->Fo
+ |Disj:Fo->Fo->Fo
+ |Impl:Fo->Fo->Fo
+.
+
+Notation " x --> y ":=(Impl x y) (at level 80).
+Notation " x -/\ y ":=(Conj x y) (at level 80).
+Notation " x -\/ y ":=(Disj x y) (at level 80).
+
+(* Substitution *)
+Fixpoint subPF (t:Fo) (xi: PropVars.t) (u : Fo): Fo.
+Proof.
+Abort. (*Defined.*)
+
+Definition Top:Fo := Impl Bot Bot.
+
+Notation " x --> y ":=(Impl x y) (at level 80).
+(* HERE *)
+Section Interpretation.
+Context (val:PropVars.t->Omega).
+Fixpoint foI (f:Fo): Omega.
+Proof.
+destruct f eqn:h.
++ exact (val p).
++ exact OFalse.
++ exact ( OAnd (foI f0_1) (foI f0_2)).
++ exact (  OOr (foI f0_1) (foI f0_2)).
++ exact ( OImp (foI f0_1) (foI f0_2)).
+Show Proof.
+Defined.
+(*
+Fixpoint foI (val:SetVars->X) (f:Fo): Omega.
+Proof.
+destruct f.
++ refine (prI p _).
+  apply (Vector.map  (teI val)).
+  exact t.
++ exact false.
++ exact ( andb (foI val f1) (foI val f2)).
++ exact (  orb (foI val f1) (foI val f2)).
++ exact (implb (foI val f1) (foI val f2)).
++  (*Infinite conjunction!!!*)
+ Show Proof.
+*)
+End Interpretation.
+
+End Formulas_mod.
