Deduction.v
@@ -21,9 +21,9 @@ Definition B1 (ps ph:Fo) (xi:SetVars) (H:isParamF xi ps = false):
  PREPR nil (ps --> ph) -> PREPR nil (ps --> Fora xi ph).
 Proof.
 intro q.
-apply MP with (A:=(Fora xi (ps --> ph))) (1:=I).
+apply MP with (A:=(Fora xi (ps --> ph))) (*1:=I*).
 (*apply (MP nil (Fora xi (ps --> ph))).*)
-+ apply (GEN) with (1:=I).
++ apply (GEN). (*with (1:=I).*)
   exact q.
 + apply (b1 _).
   exact H.
@@ -34,15 +34,15 @@ Definition gen (A:Fo) (xi:SetVars) ctx
 : PREPR ctx (A) -> PREPR ctx (Fora xi A).
 Proof.
 intro q.
-apply MP with (A:= Top) (1:=I).
+apply MP with Top.
 unfold Top.
 fold PREPR.
 exact (@AtoA ctx Bot).
-apply MP with (A:= (Fora xi (Top --> A)))  (1:=I).
-* apply GEN with (1:=I).
-  apply MP with (A:= A) (1:=I).
+apply MP with (A0:= (Fora xi (Top --> A))).
+* apply GEN.
+  apply MP with (A0:= A).
   + exact q.
-  + apply subcalc, a1.
+  + apply subcalc_OE, a1.
 * apply b1.
   trivial.
 Defined.
@@ -52,14 +52,15 @@ Definition neg (f:Fo):= (Impl f Bot).
 Definition a1i (A B : Fo)(l : list Fo):(PREPR l B)->(PREPR l (Impl A B)).
 Proof.
 intros x.
-apply MP with (A:= B) (1:=I).
+apply MP with (A0:= B).
 exact x.
-apply subcalc, a1.
+apply subcalc_OE, a1.
 Defined.
-
-Fixpoint weak (A F:Fo) (l :list Fo) (x: (PREPR l F)) : (PREPR (A::l) F).
+(*PREPR*)
+Fixpoint weak (lr:list IR) (axs:Fo -> Type)
+(A F:Fo) (l :list Fo) (x: (PR lr axs l F)) : (PR lr axs (A::l) F).
 Proof.
-destruct x as [a b|a b|i a b|a b].
+destruct x as [a b|a b|i a b] eqn:j.
 + apply hyp.
   right. (* apply inr. or_intror *)
   exact b.
@@ -69,15 +70,20 @@ apply a2.
 apply a12.
 apply b1.
 assumption. *)
-+ apply MP with (A:= a) (1:=I).
++ fold PREPR in Q.
+pose(Q2:=fun u v => weak _ _ A u _ (Q u v)).
+pose(m:=Hrule lr axs (A::l) i a b p).
+exact (m Q2).
+(*OLD
++ apply MP with (A0:= i).
   * apply weak.
     exact x1.
   * apply weak.
     exact x2.
-+ apply GEN with (1:=I). (* Order is not important! *)
-  apply weak. (* Order is not important! *)
-  exact x.
-Defined.
++ apply GEN.
+  apply weak.
+  exact x.*)
+Defined. (*(IR_MP :: IR_GEN :: Datatypes.nil) PRECA*)
 
 (*
 Fixpoint weak (A F : Fo) (l : list Fo) (x : PREPR l F) {struct x} :
@@ -97,7 +103,7 @@ destruct li.
 simpl.
 exact x.
 simpl.
-simple refine (@weak f F (li ++ l) _).
+simple refine (@weak _ _ f F (li ++ l) _).
 apply weaken.
 exact x.
 (*Show Proof.*)
@@ -107,20 +113,51 @@ Fixpoint weaken (F : Fo) (li l : list Fo) (x : PREPR l F) {struct li} :
    PREPR (li ++ l) F :=
    match li as l0 return (PREPR (l0 ++ l) F) with
    | Datatypes.nil => x
-   | f :: li0 => weak f F (li0 ++ l) (weaken F li0 l x)
+   | f :: li0 => weak _ _ f F (li0 ++ l) (weaken F li0 l x)
    end.
 
 (*Export List Notations.*)
 Fixpoint notGenWith (xi:SetVars)(l:list Fo)(B:Fo)(m:(PREPR l B)){struct m}:bool.
 Proof.
-destruct m eqn: o.
-exact true.
-destruct p eqn:j.
-exact true.
-exact true.
-exact true.
-exact (andb (notGenWith xi l _ p1) (notGenWith xi l _ p2)).
+destruct m (*eqn: o*).
++ exact true.
++ destruct p eqn:j.
+  * exact true.
+  * exact true.
+  * exact true.
++ fold PREPR in Q.
+ revert p Q . (*o*)
+  destruct u as [H|[H|H]]; try rewrite <- H; intros. clear r H.
+ simpl in * |- *.
+(*  destruct u as [H1|[H2|H3]].*)
+  3 : destruct H. (*H3*)
+  *
+(*pose (pnew:=p).
+rewrite <- H1 in pnew.
+assert(Qnew : forall u : Fo,
+    InL u (map (fun f : paramT IR_MP -> Fo => f pnew) (premi IR_MP)) ->
+    PR (IR_MP :: IR_GEN :: Datatypes.nil) PRECA l u).
+(*admit.*)
+2 : { *)
+ apply andb.
+ - unshelve eapply (notGenWith xi l (fst p)). 
+   (*fold PREPR in Qnew. ; apply Qnew.*) apply Q.
+   simpl; left; reflexivity.
+ - unshelve eapply ((notGenWith xi l (fst p --> snd p))).
+   apply Q.
+   simpl. right; left; reflexivity.
+* clear r H.
+simpl in * |- *.
+pose(xi0:=snd p).
+refine (andb (negb (SetVars.eqb xi xi0)) _).
+refine (notGenWith xi l (fst p) _ ).
+apply Q.
+left;trivial.
+(*Compute paramT IR_MP.*)
+(* OLD
+exact (andb (notGenWith xi l _ (fst p)) (notGenWith xi l _ p2)).
 exact (andb (negb (SetVars.eqb xi xi0)) (notGenWith xi l _ p) ).
+*)
 Defined.
 
 Fixpoint HA xi : true = PeanoNat.Nat.eqb (xi) (xi).
@@ -156,8 +193,17 @@ destruct m. (*as [i|i|i|i|i|i|i].*)
     (*exact (hyp _ il _ i).*)
 + apply a1i.
   apply Hax, p.
-+ apply MP with (A:= (A-->A0)) (1:=I).
++
+simpl in u. revert p Q H.
+destruct u as [Hq|[Hq|Hq]]; try rewrite <- Hq; intros. 3 : destruct Hq.
+ * (*clear r Hq.*)
+   fold PREPR in Q.
+   simpl in p,Q.
+simple refine (@Ded _ _ _ _ _).  ???
+   apply Q.
 - simple refine (@Ded _ _ _ _ _).
+{ apply Q. }    apply MP with (A-->A0).
+
   exact m1.
   intros xi H0.
   pose (W:=H xi H0).
@@ -167,7 +213,7 @@ destruct m. (*as [i|i|i|i|i|i|i].*)
   fold J.
   fold J in W.
   apply (lm _ _ W).
-- apply MP with (A:= (A-->(A0-->B))) (1:=I).
+- apply MP with (A0:= (A-->(A0-->B))).
   simple refine (@Ded _ _ _ _ _).
   exact m2.
   intros xi H0.
@@ -176,8 +222,8 @@ destruct m. (*as [i|i|i|i|i|i|i].*)
   apply (lm2 _ _ W).
  (*Last part about GEN*)
   apply a2.
-  + apply MP with (A:= (Fora xi (A-->A0))) (1:=I).
-    apply GEN with (1:=I).
+  + apply MP with (A0:= (Fora xi (A-->A0))).
+    apply GEN.
     simple refine (@Ded _ _ _ _ _).
     exact m.
     intros xi0 H0.
@@ -271,9 +317,9 @@ apply orb_intro. split. apply HB. apply HC.
 }
 unshelve eapply SimplDed. 2 : apply HB.
 unshelve eapply SimplDed. 2 : apply HA.
-apply MP with (A:=B) (1:=I). apply hyp.
+apply MP with (A0:=B). apply hyp.
 simpl. firstorder. (*apply inr.*)
-apply MP with (A:=A) (1:=I).
+apply MP with (A0:=A).
 apply hyp; firstorder.
 apply hyp; firstorder.
 Defined.
