Poly.v
@@ -1,5 +1,15 @@
-Module ModProp.
-Notation Omega := Prop.
+Module Type PolyMod.
+Parameter Omega : Type.
+Axiom OImp : Omega->Omega->Omega.
+Axiom OAnd OOr : Omega->Omega->Omega.
+Notation " x =-> y ":=(OImp x y) (at level 80).
+Notation " x =/\ y ":=(OAnd x y) (at level 80).
+Notation " x =\/ y ":=(OOr x y) (at level 80).
+End PolyMod.
+
+Module ModProp <: PolyMod.
+(*Notation Omega := Prop (only parsing).*)
+Definition Omega := Prop.
 Definition OFalse := False.
 Definition OAnd := and.
 Definition OOr := or.
@@ -7,8 +17,9 @@ Definition OImp := (fun x y:Omega => x->y).
 Notation Osig := ex.
 End ModProp.
 
-Module ModType.
-Notation Omega := Type.
+Module ModType <: PolyMod.
+(*Notation Omega := Type (only parsing).*)
+Definition Omega := Type.
 Definition OFalse := False.
 Definition OAnd := prod.
 Definition OOr := sum.
@@ -16,8 +27,9 @@ Definition OImp := (fun x y:Omega => x->y).
 Notation Osig := sigT.
 End ModType.
 
-Module ModBool.
-Notation Omega := bool.
+Module ModBool<: PolyMod.
+(*Notation Omega := bool (only parsing).*)
+Definition Omega := bool.
 Definition OFalse := false.
 Definition OAnd := andb.
 Definition OOr := orb.
